update

theory/SolverTypes.thy
@@ -1,6 +1,7 @@
 theory SolverTypes
     imports Main
-            "HOL-Library.Finite_Map"
+            "HOL-Library.RBT"
+            "StringLinorder"
 begin
 
 type_synonym BasicBlockId = string
@@ -104,32 +105,91 @@ record PcodeControlFlow =
     sucss :: "PcodeId set"
 
 record ControlFlowGraph =
-    basicblocks :: "(BasicBlockId, BasicBlockControlFlow) map"
-    pcodes :: "(PcodeId, PcodeControlFlow) map"
+    basicblocks :: "(BasicBlockId, BasicBlockControlFlow) rbt"
+    pcodes :: "(PcodeId, PcodeControlFlow) rbt"
 
 record Function =
     name :: string
     entry :: string
     exit :: string
-    basicblocks :: "(BasicBlockId, BasicBlock) map"
-    pcodes :: "(PcodeId, Pcode) map"
+    basicblocks :: "(BasicBlockId, BasicBlock) rbt"
+    pcodes :: "(PcodeId, Pcode) rbt"
     varnodes :: "Varnode list"
-    symbols :: "(SymbolId, Symbol) map"
+    symbols :: "(SymbolId, Symbol) rbt"
     cfg :: ControlFlowGraph
 
-definition mySet :: "char list set" where
-  "mySet = {''1'', ''2'', ''3''}"
+datatype Type = 
+    Integer | 
+    Bool | 
+    Float | 
+    Pointer | 
+    PointerOfPointer | 
+    Unknown
 
-(* instantiation string :: linorder
-begin
+datatype Event = 
+    ToInt | 
+    ToBool | 
+    ToFloat | 
+    ToPointer | 
+    ToPointerOfPointer | 
+    Idle
 
-end *)
+fun transition :: "Event \<Rightarrow> Type \<Rightarrow> Type" where
+    "transition ToInt Unknown = Integer" |
+    "transition ToBool Unknown = Bool" |
+    "transition ToFloat Unknown = Float" |
+    "transition ToPointer Integer = Pointer" |
+    "transition ToPointerOfPointer Pointer = PointerOfPointer" |
+    "transition _ t = t"
 
-value "sorted_list_of_set mySet"
 
+lemma "transition ToInt Unknown = Integer" by auto
+lemma "transition ToBool Unknown = Bool" by auto
+lemma "transition ToFloat Unknown = Float" by auto
+lemma "transition ToPointer Integer = Pointer" by auto
+lemma "transition ToPointerOfPointer Pointer = PointerOfPointer" by auto
+lemma "\<forall> e t. ((e \<noteq> ToInt \<and> t \<noteq> Unknown) \<and>
+            (e \<noteq> ToBool \<and> t \<noteq> Unknown) \<and>
+            (e \<noteq> ToFloat \<and> t \<noteq> Unknown) \<and>
+            (e \<noteq> ToPointer \<and> t \<noteq> Integer) \<and>
+            (e \<noteq> ToPointerOfPointer \<and> t \<noteq> Pointer)) \<longrightarrow> transition e t = t"
+proof (intro conjI allI impI)
+    fix e t
+    assume "(e \<noteq> ToInt \<and> t \<noteq> Unknown) \<and>
+            (e \<noteq> ToBool \<and> t \<noteq> Unknown) \<and>
+            (e \<noteq> ToFloat \<and> t \<noteq> Unknown) \<and>
+            (e \<noteq> ToPointer \<and> t \<noteq> Integer) \<and>
+            (e \<noteq> ToPointerOfPointer \<and> t \<noteq> Pointer)"
+    then show "transition e t = t" by (cases e) auto
+qed
 
+fun toSome :: "Type \<Rightarrow> Event" where
+    "toSome Integer = ToInt" |
+    "toSome Bool = ToBool" |
+    "toSome Float = ToFloat" |
+    "toSome Pointer = ToPointer" |
+    "toSome PointerOfPointer = ToPointerOfPointer" |
+    "toSome _ = Idle"
 
-value "''1'' @ ''2''"
-
+lemma "toSome Integer = ToInt" by auto
+lemma "toSome Bool = ToBool" by auto
+lemma "toSome Float = ToFloat" by auto
+lemma "toSome Pointer = ToPointer" by auto
+lemma "toSome PointerOfPointer = ToPointerOfPointer" by auto
+lemma "\<forall> t. (t \<noteq> Integer \<and> 
+            t \<noteq> Bool \<and>
+            t \<noteq> Float \<and>
+            t \<noteq> Pointer \<and>
+            t \<noteq> PointerOfPointer) 
+        \<longrightarrow> toSome t = Idle"
+proof (intro allI impI)
+    fix t
+    assume "t \<noteq> Integer \<and> 
+            t \<noteq> Bool \<and>
+            t \<noteq> Float \<and>
+            t \<noteq> Pointer \<and>
+            t \<noteq> PointerOfPointer"
+    then show "toSome t = Idle" by (cases t) auto
+qed
 
 end 
