theory/Solver.thy
@@ -1,0 +1,15 @@
+theory Solver
+    imports "Main"
+            "HOL-Library.RBT"
+            "SolverTypes"
+            "StringLinorder"
+begin
+
+type_synonym Context = "(Varnode, Type) rbt"
+type_synonym UDChainContext = "(PcodeId \<times> Varnode, PcodeId set) rbt"
+
+function solvePcode :: "(PcodeOp \<Rightarrow> Context \<Rightarrow> Pcode \<Rightarrow> Context) \<Rightarrow> Context \<Rightarrow> Function \<Rightarrow> PcodeId set \<Rightarrow> PcodeId \<Rightarrow> UDChainContext \<Rightarrow> (PcodeId set \<times> Context)" where
+    "solvePcode deducer ctx func visited pcodeId udChainCtx = (visited, ctx)"
+by auto
+
+end
