theory/StringLinorder.thy
@@ -1,0 +1,124 @@
+theory StringLinorder
+  imports Main
+          "HOL-Library.RBT"
+begin
+
+instantiation char :: linorder
+begin
+
+definition less_char where
+"less_char a b = (of_char a < (of_char b :: nat))"
+
+definition less_eq_char where
+"less_eq_char a b = (of_char a \<le> (of_char b :: nat))"
+
+instance by standard (auto simp add: less_char_def less_eq_char_def)
+
+end
+
+instantiation list :: (linorder) linorder
+begin
+
+fun less_eq_list where
+  "[] \<le> _ = True" |
+  "(x#xs) \<le> [] = False" |
+  "(x#xs) \<le> (y#ys) = (
+    if x = y then
+      xs \<le> ys
+    else
+      x < y
+  )"
+
+
+fun less_list where
+  "[] < ys = (ys \<noteq> [])" |
+  "(x#xs) < [] = False" |
+  "(x#xs) < (y#ys) = (
+    if x = y then
+      xs < ys
+    else
+      x < y
+  )"
+
+lemma [simp]:
+  fixes xs ys :: "'a::linorder list"
+  shows "xs \<le> ys \<or> ys \<le> xs"
+proof (induct xs arbitrary: ys)
+  case Nil
+  then show ?case by auto
+next
+  case (Cons x xs)
+  then show ?case by (induct ys) auto
+qed
+
+lemma [simp]:
+fixes xs ys zs :: "'a::linorder list"
+shows "xs \<le> ys \<Longrightarrow> ys \<le> zs \<Longrightarrow> xs \<le> zs"
+proof (induct xs arbitrary: ys zs)
+  case Nil
+  then show ?case by auto
+next
+  case (Cons x xs)
+  then show ?case
+  proof (induct ys arbitrary: zs)
+    case Nil
+    then show ?case by auto
+  next
+    case (Cons y ys)
+    then show ?case by (induct zs) auto
+  qed
+qed
+
+lemma [simp]:
+fixes xs ys :: "'a::linorder list"
+shows "xs \<le> ys \<Longrightarrow> ys \<le> xs \<Longrightarrow> xs = ys"
+proof -
+  assume "xs \<le> ys" and "ys \<le> xs"
+  then show "xs = ys"
+  proof (induct xs arbitrary: ys)
+    case Nil
+    then show ?case by (induct ys) auto
+  next
+    case (Cons x xs)
+    then show ?case by (induct ys) auto
+  qed
+qed
+
+lemma [simp]:
+fixes xs ys :: "'a::linorder list"
+shows "xs < ys = (xs \<le> ys \<and> \<not> ys \<le> xs)"
+proof (induct xs)
+  case Nil
+  then show ?case by auto
+next
+  case (Cons x xs)
+  then show ?case by (induct ys) auto
+qed
+
+instance
+proof
+  fix xs ys zs :: "'a::linorder list"
+  show "xs \<le> xs" by (induct xs) auto
+  show "xs \<le> ys \<Longrightarrow> ys \<le> zs \<Longrightarrow> xs \<le> zs" by auto
+  show "xs \<le> ys \<Longrightarrow> ys \<le> xs \<Longrightarrow> xs = ys" by auto
+  show "xs \<le> ys \<or> ys \<le> xs" by auto
+  show "xs < ys = (xs \<le> ys \<and> \<not> ys \<le> xs)" by auto
+qed
+
+end
+
+
+instantiation prod :: (linorder, linorder) linorder
+begin
+
+fun less_eq_prod :: "'a \<times> 'b \<Rightarrow> 'a \<times> 'b \<Rightarrow> bool" where
+  "(a1, b1) \<le> (a2, b2) \<longleftrightarrow> (a1 < a2) \<or> (a1 = a2 \<and> b1 \<le> b2)"
+
+fun less_prod :: "'a \<times> 'b \<Rightarrow> 'a \<times> 'b \<Rightarrow> bool" where
+  "(a1, b1) < (a2, b2) \<longleftrightarrow> (a1 < a2) \<or> (a1 = a2 \<and> b1 < b2)"
+
+instance by (standard, auto)
+
+end
+
+end
