theory/UDChain.thy
@@ -1,41 +1,85 @@
 theory UDChain
     imports "Main"
-            "HOL-Library.Finite_Map"
+            "HOL-Library.RBT"
             "SolverTypes"
+            "StringLinorder"
 begin
 
-type_synonym Context = "(PcodeId \<times> Varnode, PcodeId set) map"
+type_synonym Context = "(PcodeId \<times> Varnode, PcodeId set) rbt"
 
-function traceDefs' :: "PcodeId set \<Rightarrow> PcodeId set \<Rightarrow> Function \<Rightarrow> PcodeId \<Rightarrow> Varnode \<Rightarrow> PcodeId set" where
-    "traceDefs' visited state func pcodeId varnode = (
+fun rbt_of_list :: "('a::linorder \<times> 'b) list \<Rightarrow> ('a, 'b) rbt" where
+  "rbt_of_list [] = RBT.empty" |
+  "rbt_of_list ((k, v) # xs) = RBT.insert k v (rbt_of_list xs)"
+
+definition my_rbt :: "Context" where
+  "my_rbt = rbt_of_list [((''123'', ''123A''), empty)]"
+
+value "the (RBT.lookup my_rbt (''123'', ''123A''))"
+
+function defs' :: "PcodeId set => PcodeId set => Function => PcodeId \<Rightarrow> Varnode \<Rightarrow> PcodeId set" where
+    "defs' visited state func pcodeId varnode = (
         let visited' = insert pcodeId visited;
+            state' = insert pcodeId state;
             isAssignment = (\<lambda>pId.
-                let pcodeOpt = (pcodes func) pId
-                in case pcodeOpt of
-                    None \<Rightarrow> False |
-                    Some x \<Rightarrow> (
-                        case (pcodeOutput x) of
-                            None \<Rightarrow> False |
-                            Some _ \<Rightarrow> True));
+                    let pcodeOpt = RBT.lookup (pcodes func) pId
+                    in case pcodeOpt of
+                        None \<Rightarrow> False |
+                        Some x \<Rightarrow> (
+                            case (pcodeOutput x) of
+                                None \<Rightarrow> False |
+                                Some _ \<Rightarrow> True));
             isOutputOf = (\<lambda>vnode pId.
-                let pcodeOpt = (pcodes func) pId
-                in case pcodeOpt of
-                    None \<Rightarrow> False |
-                    Some x \<Rightarrow> (
-                        case (pcodeOutput x) of
-                            None \<Rightarrow> False |
-                            Some x' \<Rightarrow> x' = vnode));
-            nextWithState = (\<lambda>s. 
-                let pcodePredsOpt = (ControlFlowGraph.pcodes (cfg func)) pcodeId;
-                    pcodePreds = (
-                        case pcodePredsOpt of
-                            None \<Rightarrow> empty | 
-                            Some x \<Rightarrow> (PcodeControlFlow.preds x));
-                    mappedPcodePreds = map 
-                        (\<lambda>pcodeId' \<Rightarrow> traceDefs' visited' s func pcodeId' varnode) 
-                        (list_of_set pcodePreds)
-                in fold union mappedPcodePreds empty)
-        in nextWithState state)" 
+                    let pcodeOpt = RBT.lookup (pcodes func) pId
+                    in case pcodeOpt of
+                        None \<Rightarrow> False |
+                        Some x \<Rightarrow> (
+                            case (pcodeOutput x) of
+                                None \<Rightarrow> False |
+                                Some x' \<Rightarrow> x' = vnode));
+            nextWithState = (\<lambda>s :: PcodeId set. 
+                    let pcodePredsOpt = RBT.lookup (ControlFlowGraph.pcodes (cfg func)) pcodeId;
+                        pcodePreds = (
+                            case pcodePredsOpt of
+                                None \<Rightarrow> empty | 
+                                Some x \<Rightarrow> (PcodeControlFlow.preds x));
+                        mappedPcodePreds = map 
+                            (\<lambda>pcodeId' \<Rightarrow> defs' visited' s func pcodeId' varnode) 
+                            (sorted_list_of_set pcodePreds)
+                    in s)
+        in (if pcodeId \<in> visited then
+                state
+            else if isAssignment pcodeId \<and> isOutputOf varnode pcodeId then 
+                nextWithState state' 
+            else state))"
+by auto
+
+function defs :: "Context \<Rightarrow> Function \<Rightarrow> PcodeId \<Rightarrow> Varnode \<Rightarrow> (Context \<times> PcodeId set)" where
+    "defs ctx func pcodeId varnode = (
+        let containsKey = (case RBT.lookup ctx (pcodeId, varnode) of 
+                            Some _ \<Rightarrow> True | None \<Rightarrow> False);
+            defSet = (case RBT.lookup ctx (pcodeId, varnode) of
+                        Some x \<Rightarrow> x | None \<Rightarrow> empty);
+            defSet' = defs' empty empty func pcodeId varnode;
+            ctx' = RBT.insert (pcodeId, varnode) defSet' ctx
+        in (if containsKey then
+                (ctx, defSet)
+            else
+                (ctx', defSet')))"
+by auto
+
+function udChain :: "Function \<Rightarrow> Context" where
+    "udChain function = (
+        let ctx = RBT.empty;
+            pcodes = Function.pcodes function;
+            zipPcode = (\<lambda>p. map (\<lambda>x. (Pcode.id p, x)) (Pcode.inputs p));
+            targets = map (\<lambda>pId. zipPcode (the (RBT.lookup pcodes pId))) (RBT.keys pcodes);
+            targets' = concat targets
+        in foldr (\<lambda>(pId, varnode). 
+                let result = defs ctx function pId varnode;
+                    ctx' = fst result
+                in RBT.union ctx'
+            ) targets' ctx
+    )"
 by auto
 
 end
